%! Author = zero
%! Date = 29/07/2024

% Preamble
\input{preamble}

% Document
\begin{document}
    \begin{center}
        \textbf{Самостоятельная работа №4\\КНФ, ДНФ, СКНФ, СДНФ}
    \end{center}

    \begin{center}
        \textbf{Построить СКНФ, СДНФ и упростить их:}
    \end{center}

    \begin{enumerate}
        \begin{spacing}{1.5}
            \item СКНФ\\
            $\bar x \vee y$\\
            СДНФ\\
            $\bar x \wedge \bar y \vee \bar x \wedge y \vee x \wedge y = $
            $\bar x \wedge \bar y \vee y = $
            $y \vee \bar x$

            \item СКНФ\\
            $(x \vee y) \wedge (x \vee \bar y) \wedge (\bar x \vee \bar y) = $
            $(x \vee x \wedge \bar y \vee x \wedge y) \wedge (\bar x \vee y) = $
            $x \wedge (\bar x \vee \bar y) = x \wedge \bar y$\\
            СДНФ\\
            $x \wedge \bar y$

            \item СКНФ\\
            $(x \vee y \vee \bar z) \wedge (x \vee \bar y \vee z) \wedge (\bar x \vee y \vee \bar z) \wedge (\bar x \vee \bar y \vee \bar z) = $\\
            $(x \vee x \wedge \bar y \vee x \wedge z \vee x \wedge y \vee y \wedge z \vee x \wedge \bar z \vee \bar y \wedge \bar z) \wedge (\bar x \vee y \vee \bar z) \wedge (\bar x \vee \bar y \vee \bar z) = $\\
            $(x \vee y \wedge z \vee \bar y \wedge \bar z) \wedge (\bar x \vee y \vee \bar z) \wedge (\bar x \vee \bar y \vee \bar z) = $\\
            $(x \wedge y \vee x \wedge \bar z \vee \bar x \wedge y \wedge z \vee y \wedge z \vee \bar x \wedge \bar y \wedge \bar z \vee \bar y \wedge \bar z) \wedge (\bar x \vee \bar y \vee \bar z) = $\\
            $(x \wedge y \vee x \wedge \bar z \vee y \wedge z \vee \bar y \wedge \bar z) \wedge (\bar x \vee \bar y \vee \bar z) = $\\
            $x \wedge y \wedge \bar z \vee x \wedge \bar y \wedge \bar z \vee x \wedge \bar z \vee \bar x \wedge y \wedge z \vee \bar x \wedge \bar y \wedge \bar z \vee \bar y \wedge \bar z = $\\
            $x \wedge \bar z \vee \bar x \wedge y \wedge z \vee \bar y \wedge \bar z$\\
            СДНФ\\
            $\bar x \wedge \bar y \wedge \bar z \vee \bar x \wedge y \wedge z \vee x \wedge \bar y \wedge \bar z \vee x \wedge y \wedge \bar z = $\\
            $\bar x \wedge \bar y \wedge \bar z \vee x \wedge \bar y \wedge \bar z \vee \bar x \wedge y \wedge z \vee x \wedge y \wedge \bar z = $\\
            $\bar y \wedge \bar z \wedge (\bar x \vee x) \vee \bar x \wedge y \wedge z \vee x \wedge y \wedge \bar z = $\\
            $\bar y \wedge \bar z \vee \bar x \wedge y \wedge z \vee x \wedge y \wedge \bar z = $\\
            $\bar y \wedge \bar z \vee x \wedge y \wedge \bar z \vee \bar x \wedge y \wedge z = $\\
            $\bar z \wedge (\bar y \vee x \wedge y) \vee \bar x \wedge y \wedge z = $\\
            $\bar y \wedge \bar z \vee x \wedge \bar z \vee \bar x \wedge y \wedge z$
        \end{spacing}
    \end{enumerate}
\end{document}