%! Author = zero
%! Date = 29/07/2024

% Preamble
\input{preamble}

% Document
\begin{document}
    \begin{center}
        \textbf{
            Самостоятельная работа №3\\Логические аксиомы, свойства логических операций
        }

        \textbf{№1 Написать формулы}
    \end{center}

    \begin{enumerate}
        \item $x = x \wedge x$
        \item $x = x \vee x$
        \item $x = \overline {\overline x}$
        \item $x = x \wedge 1$
        \item $x = x \vee 0$
        \item $1 = x \vee 1$
        \item $1 = x \wedge \bar x$
        \item $0 = x \wedge 0$
        \item $0 = x \wedge \bar x$
    \end{enumerate}

    \begin{center}
        \textbf{№2 Упростить}
    \end{center}

    \begin{enumerate}
        \item $\overline{x \wedge y} \vee x = \bar x \vee \bar y \vee x = 1$

        \item $x \wedge (x \vee y) \vee \overline x = x \vee x \wedge y \vee \bar x = 1$
        \item $(x \vee (y \wedge z))\wedge \overline{x \vee y}) = $
        $(x \wedge y \vee x \wedge z) \wedge \overline{x \vee y} = $
        $x \wedge z \wedge (\bar x \wedge \bar y) = 0$
        \item $\overline{(\overline x \vee \overline y)} \wedge \overline x = x \wedge y \wedge \bar x = 0$
        \item $x \wedge (x \vee y) \wedge \overline{x \vee (x \wedge y)} = x \wedge (x \vee y) \wedge \bar x \wedge \overline{x \wedge y} = 0$
        \item $\overline{((x \wedge y) \vee (x \wedge z)) \wedge (\overline y \wedge \ooverline z)} = $
        \begin{spacing}{1.2}
            $\overline{(x \vee x \wedge z \vee x \wedge y \vee y \wedge z) \wedge (\bar y \wedge z)} = $
            $\overline{(x \vee y \wedge z) \wedge (\bar y \wedge z)} = $\\
            $\overline{x \wedge \bar y \wedge z} = $
            $\bar x \vee y \vee \bar z$
        \end{spacing}
    \end{enumerate}
\end{document}